rocq-skylabs-brick/tests/with_templates.v
@@ -1,6 +1,6 @@
+Require Import skylabs.prelude.base.
+Require Import skylabs.lang.cpp.syntax.
 Require Import skylabs.lang.cpp.parser.plugin.cpp2v.
-Require Import skylabs.lang.cpp.syntax.translation_unit.
-Require Import skylabs.lang.cpp.syntax.namemap.
 
 #[with_templates]
 cpp.prog templated prog cpp:{{
@@ -8,5 +8,23 @@ template <typename T> T id(T x) { return x; }
 int use() { return id<int>(3); }
 }}.
 
+Definition is_Some {T} (a : option T) : Prop :=
+  match a with
+  | Some _ => True
+  | None => False
+  end.
+
 Example has_template_symbols :
   List.length (TM.elements templated.(translation_unit.msymbols)) = 1 := eq_refl.
+
+Example id_int_exists :
+  is_Some (templated.(symbols) !! "id<int>(int)"%cpp_name).
+Proof. vm_compute. exact I. Qed.
+
+Example use_exists :
+  is_Some (templated.(symbols) !! "use()"%cpp_name).
+Proof. vm_compute. exact I. Qed.
+
+Example id_template_exists :
+  is_Some (translation_unit.msymbols templated !! "id<$T>($T)"%cpp_name).
+Proof. vm_compute. exact I. Qed.
